src/HolRefute/Refute.sml
@@ -148,6 +148,7 @@ structure Refute :> Refute = struct
   val upd_seed = Refute_Core.upd_seed
   val upd_certify = Refute_Core.upd_certify
   val upd_smart_quantifier = Refute_Core.upd_smart_quantifier
+  val upd_smart_generators = Refute_Core.upd_smart_generators
   val upd_optimise_equality = Refute_Core.upd_optimise_equality
   val upd_reorder_premises = Refute_Core.upd_reorder_premises
   val upd_mf = Refute_Core.upd_mf
